$$\pi=\sum\limits_{k=0}^\infty{\frac{1}{16^k}\left(\frac{4}{8k+1}-\frac{2}{8k+4}-\frac{1}{8k+5}-\frac{1}{8k+6}\right)}$$


$$\begin{aligned}
\int_0^{1/\sqrt2}\frac{x^{p-1}}{1-x^8}{\mathrm{d}}x&=\int_0^{1/\sqrt2}\sum\limits_{k=0}^\infty{x^{p-1+8k}}{\mathrm{d}}x\\
&=\sum_{k=0}^\infty{\int_0^{1/\sqrt2}x^{p-1+8k}\mathrm{d}x}\\
&=\sum\limits_{k=0}^\infty{\frac{2^{-4k-\frac{p}{2}}}{8k+p}}\\
&=\frac{1}{2^{p/2}}\sum\limits_{k=0}^\infty{\frac{1}{16^k}\frac{1}{8k+p}}\\
\end{aligned}$$

$$\begin{aligned}
&\sum\limits_{k=0}^\infty{\frac{1}{16^k}\left(\frac{4}{8k+1}-\frac{2}{8k+4}-\frac{1}{8k+5}-\frac{1}{8k+6}\right)}\\
=&4\cdot{2^{1/2}}\int_0^{1/\sqrt2}\frac{x^{1-1}\mathrm{d}x}{1-x^8}-2\cdot{2^{4/2}}\int_0^{1/\sqrt2}\frac{x^{4-1}\mathrm{d}x}{1-x^8}-2\cdot{2^{5/2}}\int_0^{1/\sqrt2}\frac{x^{5-1}\mathrm{d}x}{1-x^8}-2^{6/2}\int_0^{1/\sqrt2}\frac{x^{6-1}\mathrm{d}x}{1-x^8}\\
=&\int_0^{1/\sqrt2}\frac{4\sqrt2-8x^3-4\sqrt2x^4-8x^5}{1-x^8}{\mathrm{d}}x\quad\sqrt2x\to y\\
=&\int_0^1\frac{16y-16}{y^4-2y^3+4y-4}{\mathrm{d}}y\\
=&\int_0^1\frac{4y}{y^2-2}{\mathrm{d}}y-\int_0^1\frac{4y-8}{y^2-2y+2}{\mathrm{d}}y\\
=&4\left.\left[\frac{1}{2}\ln(y^2-2)\right]\right|_0^1-4\left.\left[\frac{1}{2}\ln(y^2-2y+2)+\arctan(1-y)\right]\right|_0^1\\
=&-\ln4-(-\pi-\ln4)\\
=&\pi\\
\end{aligned}$$

$$P(\color{green}{s},\color{blue}{b},\color{red}{n},A)=\sum_{k=0}^\infty\frac1{\color{blue}b^k}\sum_{j=1}^{\color{red}n}\frac{a_j}{(\color{red}nk+j)^\color{green}s}$$

$$\begin{aligned}
\pi&=\sum_{k=0}^\infty\frac1{\color{blue}{16}^k}\bigg(\frac4{(\color{red}8k+1)^\color{green}1}-\frac2{(\color{red}8k+4)^\color{green}1}-\frac1{(\color{red}8k+5)^\color{green}1}-\frac1{(\color{red}8k+6)^\color{green}1}\bigg)\\
&=P(\color{green}1,\color{blue}{16},\color{red}8,(4,0,0,−2,−1,−1,0,0))
\end{aligned}$$

$$\Phi(z,s,a)=\sum\limits_{k=0}^\infty{z^k}{(a+k)^{-s}}$$

$$\sum\limits_{k=0}^\infty{\frac{1}{b^k}\frac{1}{(j+kn)^s}}=\frac{1}{n^s}\Phi\left(\frac{1}{b},s,\frac{j}{n}\right)$$

$$\begin{aligned}
\pi&=\sum_{k=0}^{\infty}\frac{1}{16^k}\left(\frac{4}{8k+1}-\frac{2}{8k+4}-\frac{1}{8k+5}-\frac{1}{8k+6}\right)\\
16^{n}\pi&=\sum_{k=0}^{\infty}\left(\frac{4\cdot16^{k-n}}{8k+1}-\frac{2\cdot16^{k-n}}{8k+4}-\frac{16^{k-n}}{8k+5}-\frac{16^{k-n}}{8k+6}\right)
\end{aligned}$$

$$\begin{aligned}
\{16^n\pi\}&=\left\{\sum\limits_{k=0}^\infty{\left(\frac{4\cdot{16^{k-n}}}{8k+1}-\frac{2\cdot{16^{k-n}}}{8k+4}-\frac{16^{k-n}}{8k+5}-\frac{16^{k-n}}{8k+6}\right)}\right\}\\
&=\{4\{16^nS_1\}-2\{16^nS_4\}-\{16^nS_5\}-\{16^nS_6\}\}\\
\{16^nS_j\}&=\left\{\left\{\sum_{k=0}^n\frac{16^{n-k}}{8k+j}\right\}+\sum\limits_{k=n+1}^\infty{\frac{16^{n-k}}{8k+j}}\right\}\\
&=\left\{\left\{\sum_{k=0}^n\frac{16^{n-k}\quad\bmod\,8k+j}{8k+j}\right\}+\sum_{k=n+1}^\infty{\frac{16^{n-k}}{8k+j}}\right\}\\
\end{aligned}$$

$$\pi=\sum\limits_{k=0}^\infty{\left(\frac{1}{16}\right)^k}\left(\frac{8r+4}{8k+1}-\frac{8r}{8k+2}-\frac{4r}{8k+3}-\frac{8r+2}{8k+4}-\frac{2r+1}{8k+5}-\frac{2r+1}{8k+6}+\frac{r}{8k+7}\right)$$

$$\begin{aligned}
\pi&=\frac{1}{2}\sum\limits_{k=0}^\infty{\frac{1}{16^k}}\left(\frac{8}{8k+2}+\frac{4}{8k+3}+\frac{4}{8k+4}-\frac{1}{8k+7}\right)\\
\zeta(2)&=\frac{\pi^2}{6}=\frac{3}{16}\sum\limits_{k=0}^\infty{\frac{1}{64^k}}\left(\frac{16}{(6k+1)^2}-\frac{24}{(6k+2)^2}-\frac{8}{(6k+3)^2}-\frac{6}{(6k+4)^2}+\frac{1}{(6k+5)^2}\right)\\
\zeta(3)&=\frac{9}{224}\sum\limits_{k=0}^\infty{\frac{1}{4096^k}}
\left(\begin{aligned}
&\frac{1024}{(24k+2)^3}-\frac{3072}{(24k+3)^3}+\frac{512}{(24k+4)^3}+\frac{1024}{(24k+6)^3}+\frac{1152}{(24k+8)^3}\\
+&\frac{384}{(24k+9)^3}+\frac{64}{(24k+10)^3}+\frac{128}{(24k+12)^3}+\frac{16}{(24k+14)^3}+\frac{48}{(24k+15)^3}+\frac{72}{(24k+16)^3}\\
+&\frac{16}{(24k+18)^3}+\frac{2}{(24k+20)^3}-\frac{6}{(24k+21)^3}+\frac{1}{(24k+22)^3}\\
\end{aligned}\right)\\
\end{aligned}$$

$$\begin{aligned}
\operatorname{arccot}b&=\arctan{\frac{1}{b}}\\
&=\frac{1}{b}-\frac{1}{b^{3}3}+\frac{1}{b^{5}5}-\frac{1}{b^{7}7}+\frac{1}{b^{9}9}+\cdots\\
&=\sum_{k=1}^{\infty}\left[\frac{1}{b^{k}}\frac{\sin{\frac{k\pi}{2}}}{k}\right]\\
&=\frac{1}{b}\sum_{k=0}^{\infty}\left[\frac{1}{b^{4k}}\left(\frac{1}{4k+1}+\frac{-b^{-2}}{4k+3}\right)\right]\\
&=\frac{1}{b}P\left(1,b^{4},4,(1,0,-b^{-2},0)\right)\\
\ln\left(1-\frac{1}{b^m}\right)&=-\frac{1}{b^m}\sum\limits_{k=0}^\infty{\frac{1}{1+k}{b^{-mk}}}\\
&=-\frac{1}{b^m}P(1,b^m,1,(1))\\
\end{aligned}$$

$$\pi^2=\sum\limits_{k=0}^\infty{\frac{1}{\phi^{5k}}\left(\frac{\phi^{-2}}{\left(5k+1\right)^2}-\frac{\phi^{-1}}{\left(5k+2\right)^2}-\frac{\phi^{-2}}{\left(5k+3\right)^2}+\frac{\phi^{-5}}{\left(5k+4\right)^2}+\frac{2\phi^{-5}}{\left(5k+5\right)^2}\right)}$$

$$\sum\limits_{k=0}^\infty{\frac{(-1)^k}{4^k}\left(\frac{2}{4k+1}+\frac{2}{4k+2}+\frac{1}{4k+3}\right)}$$

$$\sum_{k=0}^\infty{\frac{1}{2^k}\left(\frac{a_1}{2k+1}+\frac{a_2}{2k+2}\right)}=a_2\log(2)+\sqrt2a_1\operatorname{arcsinh}(1)$$


